src/Examples/ReplicatedDisk/OneDiskAPI.v
@@ -12,16 +12,16 @@ Module OneDisk.
 
   Inductive op_step : OpSemantics Op State :=
   | step_read : forall a r state,
-      match diskGet state a with
+      match index state a with
       | Some b0 => r = b0
       | None => exists b, r = b
       end ->
       op_step (op_read a) state state r
   | step_write : forall a b state state',
-      state' = (diskUpd state a b) ->
+      state' = (assign state a b) ->
       op_step (op_write a b) state state' tt
   | step_size : forall state,
-      op_step (op_size) state state (diskSize state).
+      op_step (op_size) state state (length state).
 
   Inductive one_disk_failure : CrashSemantics State :=
   | step_id : forall (state: State), one_disk_failure state state tt.
@@ -39,7 +39,7 @@ Definition read_spec (a : addr) : Specification block unit OneDisk.State :=
     pre := True;
     post := fun state' r =>
       state' = state /\
-      diskGet state a ?|= eq r;
+      index state a ?|= eq r;
     alternate := fun state' r =>
       state' = state
   |}.
@@ -48,16 +48,16 @@ Definition write_spec (a : addr) (v : block) : Specification _ unit OneDisk.Stat
   fun state => {|
     pre := True;
     post := fun state' r =>
-      r = tt /\ state' = diskUpd state a v;
+      r = tt /\ state' = assign state a v;
     alternate := fun state' r =>
-      state' = state \/ state' = diskUpd state a v
+      state' = state \/ state' = assign state a v
   |}.
 
 Definition size_spec : Specification nat unit OneDisk.State :=
   fun state => {|
     pre := True;
     post := fun state' r =>
-      state' = state /\ r = diskSize state;
+      state' = state /\ r = length state;
     alternate := fun state' r =>
       state' = state
   |}.
